### 5.1节

2.  

> \[
> \begin{aligned}
>   &\left\| {\sin \left( {\frac{{2k\pi }}{T}x} \right)} \right\| = \left\| {\cos \left( {\frac{{2k\pi }}{T}x} \right)} \right\| = \frac{T}{2} \hfill \\
>   &f\left( x \right) = \frac{2}{T}\sum\limits_{n = 1}^\infty  {\sin \left( {\frac{{2k\pi }}{T}x} \right)\int_0^T {f\left( x \right)\sin \left( {\frac{{2k\pi }}{T}x} \right){\text{d}}x} }  \hfill \\
>    &+ \frac{2}{T}\sum\limits_{n = 1}^\infty  {\cos \left( {\frac{{2k\pi }}{T}x} \right)\int_0^T {f\left( x \right)\cos \left( {\frac{{2k\pi }}{T}x} \right){\text{d}}x} }  \hfill \\
>    &+ \frac{1}{T}\int_0^T {f\left( x \right){\text{d}}x}  \hfill \\
>    &= \frac{T}{6} + \sum\limits_{k = 1}^\infty  {\left( {\frac{T}{{3k\pi }}\sin \left( {\frac{{2k\pi }}{T}x} \right)} \right)}  \hfill \\ 
> \end{aligned}
> \]

4. 

> (1)
>
> > \[
> > \begin{aligned}
> >   \left\| {\sin \left( {2k\pi x} \right)} \right\| = \left\| {\cos \left( {2k\pi x} \right)} \right\| = \pi  \hfill \\
> >   f\left( x \right) = \int_0^{2\pi } {{{\cos }^3}x{\text{d}}x}  + \sum\limits_{k = 1}^\infty  {\sin \left( {2kx} \right)\int_0^{2\pi } {{\text{co}}{{\text{s}}^3}x\sin \left( {2kx} \right){\text{d}}x} }  \hfill \\
> >    + \sum\limits_{k = 1}^\infty  {\cos \left( {2kx} \right)\int_0^{2\pi } {{\text{co}}{{\text{s}}^3}x\cos \left( {2kx} \right){\text{d}}x} }  \hfill \\
> >    = \sum\limits_{k = 1}^\infty  {\cos \left( {2kx} \right)\int_0^{2\pi } {{\text{co}}{{\text{s}}^3}x\cos \left( {2kx} \right){\text{d}}x} }  \hfill \\
> >    =  \hfill \\ 
> > \end{aligned} 
> > \]
> >
>
> (3)
>
> > 考虑到 $f(x)$ 为偶函数，有
> > \[
> > \begin{aligned}
> >   &\int_{ - \pi }^\pi  {\cos \alpha x\cos \left( {kx} \right){\text{d}}x}  = \frac{1}{\alpha }\left( {\left. {\sin \alpha x\cos \left( {kx} \right)} \right|_{ - \pi }^\pi  + k\int_{ - \pi }^\pi  {\sin \alpha x\sin \left( {kx} \right){\text{d}}x} } \right) \hfill \\
> >   & = \frac{2}{\alpha }\sin \alpha \pi \cos k\pi  - \frac{k}{{{\alpha ^2}}}\left( {\left. {\cos \alpha x\sin \left( {kx} \right)} \right|_{ - \pi }^\pi  - k\int_{ - \pi }^\pi  {\cos \alpha x\cos \left( {kx} \right){\text{d}}x} } \right) \hfill \\
> >   & = \frac{2}{\alpha }\sin \alpha \pi \cos k\pi  + {\left( {\frac{k}{\alpha }} \right)^2}\int_{ - \pi }^\pi  {\cos \alpha x\cos \left( {2kx} \right){\text{d}}x}  \hfill \\
> >   & \Rightarrow \int_{ - \pi }^\pi  {\cos \alpha x\cos \left( {2kx} \right){\text{d}}x}  = \frac{{2\alpha }}{{{k^2} - {\alpha ^2}}}\sin \alpha \pi \cos k\pi  \hfill \\
> >  & \int_{ - \pi }^\pi  {\cos \alpha x{\text{d}}x}  = \frac{{2\sin \alpha \pi }}{\alpha } \hfill \\
> >   & \Rightarrow f\left( x \right) = \frac{1}{\pi }\sum\limits_{k = 1}^\infty  {\frac{{2{{\left( { - 1} \right)}^{k - 1}}\alpha }}{{{k^2} - {\alpha ^2}}}\sin \alpha \pi \cos \left( {kx} \right)}  + \frac{{\sin \alpha \pi }}{{\alpha \pi }} \hfill \\ 
> > \end{aligned} 
> > \]
>
> (5)
>
> > \[
> > \begin{aligned}
> >   &\int_{ - \pi }^\pi  {f\left( x \right)\cos \left( {kx} \right){\text{d}}x}  = \int_{ - \frac{\pi }{2}}^{\frac{\pi }{2}} {\cos x\cos \left( {kx} \right){\text{d}}x}  \hfill \\
> >    &= \left. {\sin x\cos \left( {kx} \right)} \right|_{ - \frac{\pi }{2}}^{\frac{\pi }{2}} + k\int_{ - \frac{\pi }{2}}^{\frac{\pi }{2}} {\sin x\sin \left( {kx} \right){\text{d}}x}  \hfill \\
> >   & = 2\cos \left( {\frac{k}{2}\pi } \right) - k\left( {\left. {\cos x\sin \left( {kx} \right)} \right|_{ - \frac{\pi }{2}}^{\frac{\pi }{2}} - k\int_{ - \frac{\pi }{2}}^{\frac{\pi }{2}} {\cos x\cos \left( {kx} \right){\text{d}}x} } \right) \hfill \\
> >   & = 2\cos \left( {k\pi } \right) + {k^2}\int_{ - \frac{\pi }{2}}^{\frac{\pi }{2}} {\cos x\cos \left( {kx} \right){\text{d}}x}  \hfill \\
> >  &  \Rightarrow \int_{ - \pi }^\pi  {f\left( x \right)\cos \left( {2kx} \right){\text{d}}x}  = \frac{{2\cos \left( {k\pi } \right)}}{{1 - {k^2}}} \hfill \\
> >  & \int_{ - \pi }^\pi  {f\left( x \right){\text{d}}x}  = 2 \hfill \\
> >   & \Rightarrow f\left( x \right) = \frac{1}{\pi }\sum\limits_{k = 1}^\infty  {\frac{{2\cos \left( {k\pi } \right)}}{{1 - {k^2}}}\cos \left( {kx} \right)}  + \frac{1}{\pi } \hfill \\ 
> > \end{aligned} 
> > \]
> >
> > 

6. 

> (1)
>
> > 首先进行偶延拓，然后求解
> > \[
> > \begin{aligned}
> >   &\int_{ - l}^l {f\left( x \right){\text{d}}x}  = \frac{{2l}}{\pi } \hfill \\
> >  & \int_{ - l}^l {f\left( x \right)\cos \left( {\frac{{k\pi x}}{l}} \right){\text{d}}x}  = \int_{ - \frac{l}{2}}^{\frac{l}{2}} {\cos \left( {\frac{{\pi x}}{l}} \right)\cos \left( {\frac{{k\pi x}}{l}} \right){\text{d}}x}  \hfill \\
> >  &  = \frac{l}{\pi }\left( {\left. {\sin \left( {\frac{{\pi x}}{l}} \right)\cos \left( {\frac{{k\pi x}}{l}} \right)} \right|_{ - \frac{l}{2}}^{\frac{l}{2}} + \frac{{k\pi }}{l}\int_{ - \frac{l}{2}}^{\frac{l}{2}} {\sin \left( {\frac{{\pi x}}{l}} \right)\sin \left( {\frac{{k\pi x}}{l}} \right){\text{d}}x} } \right) \hfill \\
> >  &  = \frac{{2l\cos \left( {\frac{{k\pi }}{2}} \right)}}{\pi } - \frac{{kl}}{\pi }\left( {\left. {\cos \left( {\frac{{\pi x}}{l}} \right)\sin \left( {\frac{{k\pi x}}{l}} \right)} \right|_{ - \frac{l}{2}}^{\frac{l}{2}} - \frac{{k\pi }}{l}\int_{ - \frac{l}{2}}^{\frac{l}{2}} {\cos \left( {\frac{{\pi x}}{l}} \right)\cos \left( {\frac{{k\pi x}}{l}} \right){\text{d}}x} } \right) \hfill \\
> >   & = \frac{{2l\cos \left( {\frac{{k\pi }}{2}} \right)}}{\pi } + {k^2}\int_{ - \frac{l}{2}}^{\frac{l}{2}} {\cos \left( {\frac{{\pi x}}{l}} \right)\cos \left( {\frac{{k\pi x}}{l}} \right){\text{d}}x}  \hfill \\
> >   & \Rightarrow \int_{ - l}^l {f\left( x \right)\cos \left( {\frac{{k\pi x}}{l}} \right){\text{d}}x}  = \frac{{2l\cos \left( {\frac{{k\pi }}{2}} \right)}}{{\left( {1 - {k^2}} \right)\pi }} \hfill \\
> >  &  \Rightarrow f\left( x \right) = \frac{1}{\pi } + \frac{1}{l}\sum\limits_{k = 1}^\infty  {\frac{{2l\cos \left( {\frac{{k\pi }}{2}} \right)}}{{\left( {1 - {k^2}} \right)\pi }}\cos \left( {\frac{{k\pi x}}{l}} \right)}  \hfill \\ 
> > \end{aligned} 
> > \]
>
> (3)
>
> > 首先进行奇延拓
> > \[
> > \int_{ - l}^l {f\left( x \right)\sin \left( {\frac{{k\pi }}{l}x} \right){\text{d}}x} 
> > \]
> > $k$ 为偶数时显然为 $0$ 
> > \[
> > 
> > \]
>
> 

8. 

> 

