$1-34$

> (1)
>
> > \[
> > V = \frac{1}{{4\pi {\varepsilon _0}r}}.\frac{4}{3}{\rho _e}\pi {R^3} = \frac{{{\rho _e}{R^3}}}{{3{\varepsilon _0}r}}
> > \]
>
> (2)
>
> > \[
> > V = \frac{{{\rho _e}{R^2}}}{{3{\varepsilon _0}}}
> > \]
>
> (3)
>
> > \[
> > \begin{gathered}
> >   \vec E = \frac{4}{3}{\rho _e}\pi {r^3}\frac{1}{{4\pi {\varepsilon _0}{r^2}}} = \frac{{{\rho _e}r}}{{3{\varepsilon _0}}} \hfill \\
> >   V = \frac{{{\rho _e}{R^2}}}{{3{\varepsilon _0}}} - \int_R^r {\frac{{{\rho _e}r'}}{{3{\varepsilon _0}}}{\text{d}}r'}  = \frac{{{\rho _e}{R^2}}}{{3{\varepsilon _0}}} - \left( {\frac{{{\rho _e}{r^2}}}{{6{\varepsilon _0}}} - \frac{{{\rho _e}{R^2}}}{{6{\varepsilon _0}}}} \right) = \frac{{{\rho _e}{R^2}}}{{2{\varepsilon _0}}} - \frac{{{\rho _e}{r^2}}}{{6{\varepsilon _0}}} \hfill \\ 
> > \end{gathered} 
> > \]

$1-36$

> (1)
>

$1.37$

> 以无穷远点为势能零点
> \[
> \begin{gathered}
>   \vec E = \left\{ \begin{gathered}
>   \frac{{{\rho _e}r}}{{2{\varepsilon _0}}}\quad r \leqslant R \hfill \\
>   \frac{{{\rho _e}{R^2}}}{{2{\varepsilon _0}r}}\quad r > R \hfill \\ 
> \end{gathered}  \right. \hfill \\
>   V =  - \int_0^r {\vec E \cdot {\text{d}}\vec r}  = \left\{ \begin{gathered}
>   \frac{{{\rho _e}{r^2}}}{{4{\varepsilon _0}}} \hfill \\
>   \frac{{{\rho _e}{R^2}}}{{4{\varepsilon _0}}} + \frac{{{\rho _e}{R^2}}}{{2{\varepsilon _0}}}\ln \frac{r}{R} \hfill \\ 
> \end{gathered}  \right. \hfill \\ 
> \end{gathered} 
> \]

$1-43$

> \[
> \begin{gathered}
>   {V_B} = \int_{ - \frac{l}{2}}^{\frac{l}{2}} {\frac{1}{{4\pi {\varepsilon _0}}}\frac{{{l_e}{\text{d}}x}}{{\sqrt {{{\left( {\frac{x}{2}} \right)}^2} + {b^2}} }}}  \hfill \\
>    = \int_{ - \arctan \frac{l}{{4b}}}^{\arctan \frac{l}{{4b}}} {\frac{1}{{2\pi {\varepsilon _0}}}\frac{{{l_e}}}{{\cos \theta }}{\text{d}}\theta }  \hfill \\
>    =  - \int_{ - \arctan \frac{l}{{4b}}}^{\arctan \frac{l}{{4b}}} {\frac{1}{{2\pi {\varepsilon _0}}}\frac{{{l_e}}}{{1 - {{\sin }^2}\theta }}{\text{dsin}}\theta }  \hfill \\
>    =  - \frac{1}{{2\pi {\varepsilon _0}}}\frac{{{l_e}}}{2}\left. {\ln \left( {\frac{{1 + x}}{{1 - x}}} \right)} \right|_{x =  - \frac{l}{{\sqrt {16{b^2} + {l^2}} }}}^{x = \frac{l}{{\sqrt {16{b^2} + {l^2}} }}} \hfill \\
>    =  - \frac{{{l_e}}}{{2\pi {\varepsilon _0}}}\left. {\ln \left( {\frac{{1 + x}}{{1 - x}}} \right)} \right|_{x =  - \frac{l}{{\sqrt {16{b^2} + {l^2}} }}}^{x = \frac{l}{{\sqrt {16{b^2} + {l^2}} }}} \hfill \\ 
> \end{gathered} 
> \]

$1-49$

> 